proofs/hol_light/aarch64/proofs/mldsa_polyz_unpack_consts.ml
@@ -1,0 +1,39 @@
+(*
+ * Copyright Amazon.com, Inc. or its affiliates. All Rights Reserved.
+ * SPDX-License-Identifier: Apache-2.0 OR ISC OR MIT-0
+ *)
+
+(*
+ * WARNING: This file is auto-generated from scripts/autogen
+ *          in the mldsa-native repository.
+ *          Do not modify it directly.
+ *)
+
+(*
+ * TBL index tables for polyz_unpack_{17,19}
+ * See autogen for details.
+ *)
+
+let mldsa_polyz_unpack_17_indices = (REWRITE_RULE[MAP] o define)
+  `mldsa_polyz_unpack_17_indices:byte list = MAP word [
+    0;   1;   2; 255;   2;   3;   4; 255;
+    4;   5;   6; 255;   6;   7;   8; 255;
+    9;  10;  11; 255;  11;  12;  13; 255;
+   13;  14;  15; 255;  15;  16;  17; 255;
+    2;   3;   4; 255;   4;   5;   6; 255;
+    6;   7;   8; 255;   8;   9;  10; 255;
+   11;  12;  13; 255;  13;  14;  15; 255;
+   15;  28;  29; 255;  29;  30;  31; 255
+]`;;
+
+let mldsa_polyz_unpack_19_indices = (REWRITE_RULE[MAP] o define)
+  `mldsa_polyz_unpack_19_indices:byte list = MAP word [
+    0;   1;   2; 255;   2;   3;   4; 255;
+    5;   6;   7; 255;   7;   8;   9; 255;
+   10;  11;  12; 255;  12;  13;  14; 255;
+   15;  16;  17; 255;  17;  18;  19; 255;
+    4;   5;   6; 255;   6;   7;   8; 255;
+    9;  10;  11; 255;  11;  12;  13; 255;
+   14;  15;  24; 255;  24;  25;  26; 255;
+   27;  28;  29; 255;  29;  30;  31; 255
+]`;;
